prove mp_wf_prime

LeanChecker/Proof.lean
@@ -1,5 +1,8 @@
 import LeanChecker.Pattern
 import Mathlib.Tactic.Contrapose
+import Mathlib.Tactic.LibrarySearch
+import Mathlib.Tactic.Propose
+import Mathlib.Tactic.GCongr
 
 inductive Proof where
     | instantiate(schema: Proof)(subst: Nat -> Option Pattern) : Proof /-- TODO: We need simultanous substitutions here --/
@@ -19,7 +22,7 @@ def prop2_concl := (implies (implies ph0 (implies ph1 ph2)) (implies (implies ph
 def mp_conclusion(hyp1: Option Pattern)(hyp2: Option Pattern) : Option Pattern := match (hyp1, hyp2) with
           | (none, _) => none
           | (_, none) => none
-          | (some concl_1, some (Pattern.implies concl_2_left concl_2_right)) =>
+          | (some (Pattern.implies concl_2_left concl_2_right), some concl_1) =>
                 if concl_2_left = concl_1 then concl_2_right else none
           | (some _, some _) => none
 
@@ -32,7 +35,9 @@ def Proof.conclusion(pi: Proof) : Option Pattern :=
           | some concl' => (concl'.instantiate subst')
       | Proof.prop1 => prop1_concl
       | Proof.prop2 => prop2_concl
-      | Proof.modus_ponens pi1 pi2 => mp_conclusion pi2.conclusion  pi1.conclusion
+      | Proof.modus_ponens pi1 pi2 => mp_conclusion pi1.conclusion  pi2.conclusion
+
+---
 
 def imp_refl: Proof :=
     (mp (inst (mp (inst prop2 $ subst_from_pairs [(2, ph0)])
@@ -42,7 +47,9 @@ def imp_refl: Proof :=
         (inst prop1 $ subst_from_pairs [(1, ph0)])
     )
 
-theorem test_imp_refl : imp_refl.conclusion = some ph0_implies_ph0 := by rfl
+example : imp_refl.conclusion = some ph0_implies_ph0 := by rfl
+
+---
 
 def merge_instantiation(inner: Nat -> Option Pattern)(outer: Nat -> Option Pattern)
  : Nat -> Option Pattern :=
@@ -50,23 +57,109 @@ def merge_instantiation(inner: Nat -> Option Pattern)(outer: Nat -> Option Patte
     | none => outer n
     | some p => some $ p.instantiate outer
 
+@[simp]
 def push_instantiations(p: Proof) : Proof :=
     match p with
     | Proof.prop1 => p
     | Proof.prop2 => p
+    | (Proof.modus_ponens l r) => (Proof.modus_ponens (push_instantiations l) (push_instantiations r))
     | (Proof.instantiate Proof.prop1 _)  => p
     | (Proof.instantiate Proof.prop2 _)  => p
-    | (Proof.modus_ponens l r) => (Proof.modus_ponens (push_instantiations l) (push_instantiations r))
     | (Proof.instantiate (Proof.modus_ponens l' r') subst)
          => (Proof.modus_ponens (push_instantiations (Proof.instantiate l' subst))
                                 (push_instantiations (Proof.instantiate r' subst)))
     | (Proof.instantiate (Proof.instantiate p' subst_inner) subst_outer)
-         => (Proof.instantiate p'  (merge_instantiation subst_inner subst_outer))
+         => (push_instantiations (Proof.instantiate p'  (merge_instantiation subst_inner subst_outer)))
+
+
+example : (push_instantiations imp_refl).conclusion = some ph0_implies_ph0 := by rfl
 
 
 
 @[simp]
 def Proof.wf(p: Proof) : Bool := p.conclusion != none
+
+
+
+
+theorem mp_wf_prime : (Proof.modus_ponens l r).conclusion = some psi
+                         -> ∃ phi, r.conclusion = some phi ∧ l.conclusion = (some $ Pattern.implies phi psi) :=
+by
+   simp
+   split
+   case h_1 => simp
+   case h_2 => simp
+   case h_3 concl_2_left concl_2_right concl_1 heq
+    => split
+       case inl h => intro a
+                     use concl_2_left
+                     simp at heq; simp at a
+                     exact ⟨ by simp [heq.2, h], by simp[heq, <- a]⟩
+       case inr => simp
+   case h_4 => simp
+
+theorem mp_wf : (Proof.modus_ponens l r).wf -> l.wf ∧ r.wf :=
+    by {
+        generalize h_left_conc: l.conclusion = lconc
+        generalize h_right_conc: r.conclusion = rconc
+        match lconc with
+        | none  => simp [h_left_conc, h_right_conc]
+        | some (Pattern.implies phi psi)  => {
+            match rconc with
+            | none => simp [h_left_conc, h_right_conc]
+
+            | some phi' => { apply @Classical.byCases (phi = phi')
+                             . intro
+                               simp [h_left_conc, h_right_conc]
+                             . intro
+                               simp[h_left_conc, h_right_conc]
+                           }
+        }
+        | some Pattern.bot  => cases rconc <;> simp[h_left_conc, h_right_conc]
+        | some (Pattern.metavar _)  => cases rconc <;> simp[h_left_conc, h_right_conc]
+    }
+
+theorem instantiate_wf : (Proof.instantiate p' subst).wf -> p'.wf := sorry
+theorem instantiate_wf_inv : p'.wf -> (Proof.instantiate p' subst).wf  := sorry
+
+
+theorem instantiate_commutes_with_implies(left: Pattern)(right: Pattern)(subst: Nat -> Option Pattern)
+    : ((Pattern.implies left right).instantiate subst) = (Pattern.implies (left.instantiate subst) (right.instantiate subst))
+    := by rw [Pattern.instantiate]
+
+theorem instantiate_commutes_with_mp(left: Proof)(right: Proof)(subst: Nat -> Option Pattern)
+     (h_left_conc : left.conclusion = (Pattern.implies phi psi))
+     (h_right_conc : right.conclusion = some phi):
+      (Proof.instantiate (Proof.modus_ponens left right) subst).conclusion
+    = (Proof.modus_ponens (Proof.instantiate left subst) (Proof.instantiate right subst)).conclusion
+    := by {
+    simp [  mp_conclusion, h_right_conc, h_left_conc, instantiate_commutes_with_implies]
+    }
+
+
+theorem xxx (p: Proof) (p_has_conclusion : p.wf) :
+    (push_instantiations p).conclusion = p.conclusion := by
+    induction p with
+    | prop1 => rfl
+    | prop2 => rfl
+    | modus_ponens l r pl pr =>
+        rw [(mp_wf p_has_conclusion).1] at pl
+        simp at pl
+        rw [(mp_wf p_has_conclusion).2] at pr
+        simp at pr
+        simp [pl, pr]
+
+    | instantiate p' subst h' =>
+        have pp_has_concl : p'.wf := instantiate_wf p_has_conclusion
+        rw [pp_has_concl] at h'
+        cases p' with
+        | prop1 => rfl
+        | prop2 => rfl
+        | modus_ponens l r =>
+            simp at h'
+            unfold push_instantiations
+            have xxx := (mp_wf pp_has_concl).1
+
 
 
 def Proof.is_instantiated_schema(p: Proof) : Bool :=
@@ -87,37 +180,3 @@ def Proof.is_pre_instantiated(p: Proof) : Bool :=
     match p with
     | (Proof.modus_ponens p1 p2) => p1.is_pre_instantiated ∧ p2.is_pre_instantiated
     | _  => p.is_instantiated_schema ∧ p.conclusion.isSome
-
-def mp_wf_left : (Proof.modus_ponens l r).wf -> l.wf ∧ r.wf :=
-    by {
-        generalize h_left_conc: l.conclusion = lconc
-        generalize h_right_conc: r.conclusion = rconc
-        match rconc with
-        | none  => simp [h_left_conc, h_right_conc]
-        | some (Pattern.implies phi psi)  => {
-            match lconc with
-            | none => simp [h_left_conc, h_right_conc]
-
-            | some phi' => { apply @Classical.byCases (phi = phi')
-                             . intro
-                               simp [h_left_conc, h_right_conc]
-                             . intro
-                               simp[h_left_conc, h_right_conc]
-                           }
-        }
-        | some Pattern.bot  => cases lconc <;> simp[h_left_conc, h_right_conc]
-        | some (Pattern.metavar _)  => cases lconc <;> simp[h_left_conc, h_right_conc]
-    }
-
-theorem instantiate_commutes_with_implies(left: Pattern)(right: Pattern)(subst: Nat -> Option Pattern)
-    : ((Pattern.implies left right).instantiate subst) = (Pattern.implies (left.instantiate subst) (right.instantiate subst))
-    := by rw [Pattern.instantiate]
-
-theorem instantiate_commutes_with_mp(left: Proof)(right: Proof)(subst: Nat -> Option Pattern)
-     (h_left_conc : left.conclusion = (Pattern.implies phi psi))
-     (h_right_conc : right.conclusion = some phi):
-      (Proof.instantiate (Proof.modus_ponens left right) subst).conclusion
-    = (Proof.modus_ponens (Proof.instantiate left subst) (Proof.instantiate right subst)).conclusion
-    := by {
-    simp [  mp_conclusion, h_right_conc, h_left_conc, instantiate_commutes_with_implies]
-    }
