LeanChecker/Pattern.lean
@@ -28,13 +28,8 @@ def Pattern.instantiate(p: Pattern)(subst: Nat -> Option Pattern) : Pattern :=
       | Pattern.bot => Pattern.bot
       | Pattern.implies left right => Pattern.implies (left.instantiate subst) (right.instantiate subst)
 
-theorem test_inst_1 :
-    (Pattern.instantiate Pattern.bot  $ subst_from_pairs [(0, ph0)]) = Pattern.bot := by rfl
-theorem test_inst_2 :
-    (Pattern.instantiate ph0 $ subst_from_pairs [(0, ph0)]) = ph0 := by rfl
-theorem test_inst_3 :
-    (Pattern.instantiate ph1 $ subst_from_pairs [(0, ph0)]) = ph1 := by rfl
-theorem test_inst_4 :
-    (Pattern.instantiate ph0_implies_ph0 $ subst_from_pairs [(0, ph1)]) = (implies ph1 ph1) := by rfl
-theorem test_inst_5 :
-    (Pattern.instantiate ph0_implies_ph0 $ subst_from_pairs [(0, ph0_implies_ph0)]) = (implies ph0_implies_ph0 ph0_implies_ph0) := by rfl
+example : (Pattern.instantiate Pattern.bot  $ subst_from_pairs [(0, ph0)]) = Pattern.bot := by rfl
+example : (Pattern.instantiate ph0 $ subst_from_pairs [(0, ph0)]) = ph0 := by rfl
+example : (Pattern.instantiate ph1 $ subst_from_pairs [(0, ph0)]) = ph1 := by rfl
+example : (Pattern.instantiate ph0_implies_ph0 $ subst_from_pairs [(0, ph1)]) = (implies ph1 ph1) := by rfl
+example : (Pattern.instantiate ph0_implies_ph0 $ subst_from_pairs [(0, ph0_implies_ph0)]) = (implies ph0_implies_ph0 ph0_implies_ph0) := by rfl
